Update the demo

tests/fstar/demo/Demo.fst
@@ -28,14 +28,19 @@ let use_mul2_add1 (x : u32) (y : u32) : result u32 =
 let incr (x : u32) : result u32 =
   u32_add x 1
 
+(** [demo::use_incr]:
+    Source: 'src/demo.rs', lines 25:0-25:17 *)
+let use_incr : result unit =
+  let* i = incr 0 in let* i1 = incr i in let* _ = incr i1 in Return ()
+
 (** [demo::CList]
-    Source: 'src/demo.rs', lines 27:0-27:17 *)
+    Source: 'src/demo.rs', lines 34:0-34:17 *)
 type cList_t (t : Type0) =
 | CList_CCons : t -> cList_t t -> cList_t t
 | CList_CNil : cList_t t
 
 (** [demo::list_nth]:
-    Source: 'src/demo.rs', lines 32:0-32:56 *)
+    Source: 'src/demo.rs', lines 39:0-39:56 *)
 let rec list_nth (t : Type0) (n : nat) (l : cList_t t) (i : u32) : result t =
   if is_zero n
   then Fail OutOfFuel
@@ -48,7 +53,7 @@ let rec list_nth (t : Type0) (n : nat) (l : cList_t t) (i : u32) : result t =
     end
 
 (** [demo::list_nth_mut]:
-    Source: 'src/demo.rs', lines 47:0-47:68 *)
+    Source: 'src/demo.rs', lines 54:0-54:68 *)
 let rec list_nth_mut
   (t : Type0) (n : nat) (l : cList_t t) (i : u32) :
   result (t & (t -> result (cList_t t)))
@@ -74,7 +79,7 @@ let rec list_nth_mut
     end
 
 (** [demo::list_nth_mut1]: loop 0:
-    Source: 'src/demo.rs', lines 62:0-71:1 *)
+    Source: 'src/demo.rs', lines 69:0-78:1 *)
 let rec list_nth_mut1_loop
   (t : Type0) (n : nat) (l : cList_t t) (i : u32) :
   result (t & (t -> result (cList_t t)))
@@ -99,7 +104,7 @@ let rec list_nth_mut1_loop
     end
 
 (** [demo::list_nth_mut1]:
-    Source: 'src/demo.rs', lines 62:0-62:77 *)
+    Source: 'src/demo.rs', lines 69:0-69:77 *)
 let list_nth_mut1
   (t : Type0) (n : nat) (l : cList_t t) (i : u32) :
   result (t & (t -> result (cList_t t)))
@@ -107,7 +112,7 @@ let list_nth_mut1
   let* (x, back_'a) = list_nth_mut1_loop t n l i in Return (x, back_'a)
 
 (** [demo::i32_id]:
-    Source: 'src/demo.rs', lines 73:0-73:28 *)
+    Source: 'src/demo.rs', lines 80:0-80:28 *)
 let rec i32_id (n : nat) (i : i32) : result i32 =
   if is_zero n
   then Fail OutOfFuel
@@ -117,21 +122,41 @@ let rec i32_id (n : nat) (i : i32) : result i32 =
     then Return 0
     else let* i1 = i32_sub i 1 in let* i2 = i32_id n1 i1 in i32_add i2 1
 
+(** [demo::list_tail]:
+    Source: 'src/demo.rs', lines 88:0-88:64 *)
+let rec list_tail
+  (t : Type0) (n : nat) (l : cList_t t) :
+  result ((cList_t t) & (cList_t t -> result (cList_t t)))
+  =
+  if is_zero n
+  then Fail OutOfFuel
+  else
+    let n1 = decrease n in
+    begin match l with
+    | CList_CCons x tl ->
+      let* (c, list_tail_back) = list_tail t n1 tl in
+      let back_'a =
+        fun ret -> let* tl1 = list_tail_back ret in Return (CList_CCons x tl1)
+        in
+      Return (c, back_'a)
+    | CList_CNil -> Return (CList_CNil, Return)
+    end
+
 (** Trait declaration: [demo::Counter]
-    Source: 'src/demo.rs', lines 83:0-83:17 *)
+    Source: 'src/demo.rs', lines 97:0-97:17 *)
 noeq type counter_t (self : Type0) = { incr : self -> result (usize & self); }
 
 (** [demo::{(demo::Counter for usize)}::incr]:
-    Source: 'src/demo.rs', lines 88:4-88:31 *)
+    Source: 'src/demo.rs', lines 102:4-102:31 *)
 let counterUsize_incr (self : usize) : result (usize & usize) =
   let* self1 = usize_add self 1 in Return (self, self1)
 
 (** Trait implementation: [demo::{(demo::Counter for usize)}]
-    Source: 'src/demo.rs', lines 87:0-87:22 *)
+    Source: 'src/demo.rs', lines 101:0-101:22 *)
 let counterUsize : counter_t usize = { incr = counterUsize_incr; }
 
 (** [demo::use_counter]:
-    Source: 'src/demo.rs', lines 95:0-95:59 *)
+    Source: 'src/demo.rs', lines 109:0-109:59 *)
 let use_counter
   (t : Type0) (counterInst : counter_t t) (cnt : t) : result (usize & t) =
   counterInst.incr cnt
